test/oneoff/specialization_plan/ExternSemanticStrength.v
@@ -15,9 +15,9 @@ Definition empty_extern_downstream : Semantics :=
      sem_arguments_represent := fun _ _ _ _ => True;
      sem_represents := fun _ _ _ _ => True;
      sem_sail_eval := fun _ _ _ => True;
-     sem_jib_eval := fun _ _ _ => False;
-     sem_conversion_eval := fun _ _ _ _ _ => False;
-     sem_call_arguments_represent := fun _ _ _ => True;
+     sem_jib_eval := fun _ _ _ => True;
+     sem_conversion_eval := fun _ _ _ _ _ => True;
+     sem_call_arguments_represent := fun _ _ _ => False;
      sem_sail_call := fun _ _ _ _ => True;
      sem_jib_call := fun _ _ _ _ _ => False;
      sem_extern_eval := fun _ _ _ => False;
@@ -31,14 +31,27 @@ Theorem extern_requires_execution :
   ~ obligation_4e81ef1ad207ac8ec4288e2a2826812a empty_extern_downstream.
 Proof.
   intro obligation.
-  destruct (obligation [] [] tt I I) as [extern_outcome [extern_execution _]].
-  exact extern_execution.
+  destruct (obligation [] tt I)
+    as [represented_args [extern_outcome [call_representation _]]].
+  exact call_representation.
 Qed.
 
 Theorem extern_call_requires_jib_execution :
   ~ obligation_957a1e45102c495c424852247c6bd899 empty_extern_downstream.
 Proof.
   intro obligation.
-  destruct (obligation [] [] tt I I) as [jib_outcome [jib_call _]].
-  exact jib_call.
+  destruct (obligation [] tt I)
+    as [represented_args [jib_outcome [call_representation _]]].
+  exact call_representation.
+Qed.
+
+Theorem complete_requires_extern_call_representation :
+  ~ Complete empty_extern_downstream.
+Proof.
+  intro complete.
+  destruct
+    (proof_4e81ef1ad207ac8ec4288e2a2826812a
+      empty_extern_downstream complete [] tt I)
+    as [represented_args [extern_outcome [call_representation _]]].
+  exact call_representation.
 Qed.
